u = \frac{x C_5 - \frac{x^2 p_1}{2} - \frac{x^3 \Delta p}{6 l}}{E A} + C_6

w = \frac{\frac{x^4 q_1}{24} 
  + \frac{\frac{x^4 \Delta m}{24} + \frac{x^5 \Delta q}{120}}{l}}{J E} + \frac{x^3 C_1}{6} 
      + \frac{x^2 C_2}{2} + x C_3 + C_4

\theta 
  = \frac{\frac{x^4 \Delta q + 4 x^3 \Delta m}{l} + 4 x^3 q_1}{-24 J E} - C_3 
      - \frac{x^2 C_1}{2} - x C_2

N = C_5 - x p_1 - \frac{x^2 \Delta p}{2 l}

T = m_1 - E J C_1 - x q_1 - \frac{x^2 \Delta q}{2 l}

M = -\frac{\frac{x^3 \Delta q}{6} + \frac{x^2 \Delta m}{2}}{l} - E J  (C_2 + x C_1) 
      - \frac{x^2 q_1}{2}
