u = \frac{1}{E A} \left( C_5 x - \frac{p_1}{2} x^2 - \frac{\Delta p}{6 l}x^3 \right) + C_6

w = \frac{\frac{\frac{\Delta q}{120} x^5 + \frac{Dm}{24} x^4}{E J} 
  - \frac{\chi \Delta q}{6 G A}x^3}{l} + \frac{q_1}{24 E J} x^4 - \frac{C_1}{6} x^3 
      - \frac{ C_2 + \frac{\chi q_1}{G A} }{2} x^2  + C_3 x + C_4

\theta 
  = \frac{\chi  (E J C_1 + m_1)}{A G} + C_2 x + \frac{C_1}{2} x^2 
      - \frac{4 x^3 q_1 + \frac{x^4 \Delta q + 4 x^3 Dm}{l}}{24 J E} - C_3

N = - \frac{\Delta p}{2 l} x^2 - p_1 x + C_5 

T = - \frac{\Delta q}{2 l} x^2 - x q_1 + E J C_1 + m_1 

M = - \frac{\Delta q}{6l}x^3 - \left( \frac{q_1}{2} + \frac{\Delta m}{2l} \right) x^2 + E J  (x C_1 + C_2) 
